erasing memoization (almost) work (still one unecessary assume)

examples/dm4free/ml/FStar_Erase_Heap_ST.ml
@@ -6,7 +6,11 @@ type inductive_inv = heap -> Obj.t
 
 type (_,_,_,_,_,_,_,_) invariant = unit
 
-let erase_st: type a b wp. (a -> (b, wp) _dm4f_STATE_repr) -> a -> b =
-  fun f ->
-  let r = ref emp in
-  fun x -> let y, h = f x !r in r := h ; y
+type ('a,_) erase_initializer = unit -> ('a, Obj.t) _dm4f_STATE_repr
+
+let erase_st: type a b r inv wp. (r -> a -> (b, wp) _dm4f_STATE_repr) -> (r, inv) erase_initializer -> a -> b =
+  fun f init ->
+  let r0, h0 = init () emp in
+  let r = ref h0 in
+  let f' = f r0 in
+  fun x -> let y, h = f' x !r in r := h ; y
