examples/dm4free/FStar.Erase.Heap.ST.fst
@@ -4,7 +4,7 @@ open FStar.DM4F.Heap
 open FStar.DM4F.Heap.ST
 
 
-let inductive_inv = p:(heap -> Type0){ p emp }
+let inductive_inv = p:(heap -> Type0)
 
 let invariant (#a #b:Type)
   (p:inductive_inv) (pre_pure:a -> pure_pre) (post_pure:a -> pure_post b)
@@ -15,11 +15,17 @@ let invariant (#a #b:Type)
   (* The result of f does not depend on the initial state as long as it satisfies the invariant *)
   (forall s1 s2. p s1 /\ p s2 ==> (forall x. pre_pure x ==> fst (reify (f x) s1) == fst (reify (f x) s2)))
 
-let erase_st (#a #b:Type)
-    (p:inductive_inv) (pre_pure:a -> pure_pre) (post_pure:a -> pure_post b)
-    (#pre:a -> st_pre) (#post:a -> st_post b) (f: x:a -> ST b (pre x) (post x))
+let erase_initializer (#a:Type) (p:a -> inductive_inv) = unit -> ST a (requires (fun _ -> True)) (ensures (fun _ r h -> p r h))
+
+let erase_st (#a #b #r:Type)
+    (p:r -> inductive_inv) (pre_pure:a -> pure_pre) (post_pure:a -> pure_post b)
+    (#pre:r -> a -> st_pre) (#post:r -> a -> st_post b) (f: r0:r -> Tot (x:a -> ST b (pre r0 x) (post r0 x)))
+    (init:erase_initializer p)
   : Pure (x:a -> Pure b (pre_pure x) (post_pure x))
-    (requires (invariant p pre_pure post_pure #pre #post f))
-      (ensures (fun g -> (invariant p pre_pure post_pure #pre #post f) /\
-                      (forall x. pre_pure x ==> g x == fst (reify (f x) emp))))
-= fun (x:a) -> fst (reify (f x) emp)
+    (requires (forall r. invariant (p r) pre_pure post_pure #(pre r) #(post r) (f r)))
+      (ensures (fun g -> let r, h0 = reify (init ()) emp in
+                      (invariant (p r) pre_pure post_pure #(pre r) #(post r) (f r)) /\
+                      (forall x. pre_pure x ==> g x == fst (reify (f r x) h0))))
+= let r, h0 = reify (init ()) emp in
+  let f' = f r in
+  fun (x:a) -> fst (reify (f' x) h0)
