examples/dm4free/FStar.Erase.Test.fst
@@ -1,11 +1,104 @@
+module FStar.Erase.Test
+
+open FStar.DM4F.Heap
 open FStar.DM4F.Heap.ST
 open FStar.Erase.Heap.ST
+module L = FStar.List.Tot
 
+(* let h (pre:st_pre) (post:st_post unit) (f: unit -> ST unit pre post) (h:heap) = *)
+(*   let g () : Lemma (fst (reify (f ())) h == ()) = () in *)
+(*   () *)
 
-let memo (#a:eqtype) (#b:Type) (f:a -> Tot b) () : ST (a -> ST b) =
-  let r = alloc #(list (a * b)) [] in
-  let g (x:a) : ST b =
+let memo_t (a:eqtype) (b:Type) = ref (list (a * b))
+
+(* ******************************************************************************** *)
+(*                                  Taken from Memo                                 *)
+(* ******************************************************************************** *)
+
+let rec for_all_prop (#a:Type) (p:a -> Type0) (l:list a) : Tot Type0 (decreases l)
+= match l with
+  | [] -> True
+  | x :: xs -> p x /\ for_all_prop p xs
+
+let rec for_all_prop_assoc_lemma (#a:eqtype) (#b:Type) (x:a) (p : (a * b) -> Tot Type0) (l:list (a*b))
+  : Lemma (requires (for_all_prop p l))
+    (ensures (match L.assoc x l with Some y -> p (x,y) | _ -> True))
+= match l with
+  | [] -> ()
+  | (x0, y0) :: xs -> if x0 = x then () else for_all_prop_assoc_lemma x p xs
+
+let forall_prop_assoc_lemma2 (#a:eqtype) (#b:Type) (x:a) (y:b) (p : (a * b) -> Tot Type0)
+  : Lemma (forall h. for_all_prop p h /\ List.assoc x h == Some y ==> p (x,y))
+= let aux h : Lemma (requires (for_all_prop p h /\ List.assoc x h == Some y)) (ensures (p (x,y))) =
+      for_all_prop_assoc_lemma x p h
+  in
+  FStar.Classical.(forall_intro (move_requires aux))
+
+let valid_memo (#a:eqtype) (#b:Type) (h:list (a * b)) (f:a -> Tot b) =
+  for_all_prop (fun (x,y) -> y == f x) h
+
+let memo_invariant (#a:eqtype) (#b:Type) (f: a -> Tot b) (r:memo_t a b) : inductive_inv =
+  fun (h:heap) ->
+    h `contains_a_well_typed` r /\
+    valid_memo (sel h r) f
+
+let memo_initializer (#a:eqtype) (#b:Type) (f:a -> Tot b)
+  : erase_initializer (memo_invariant f)
+= fun () -> alloc []
+
+let memo (#a:eqtype) (#b:Type) (f:a -> Tot b) (r:memo_t a b) : Tot (x:a -> ST b (requires (memo_invariant f r)) (ensures (fun _ y h1 -> memo_invariant f r h1 /\ y == f x))) =
+  let g (x:a) : ST b (requires (memo_invariant f r)) (ensures (fun _ y h1 -> memo_invariant f r h1 /\ y == f x)) =
     match L.assoc x !r with
+    | Some y ->
+      forall_prop_assoc_lemma2 x y (fun (x,y) -> y == f x) ;
+      y
     | None -> let y = f x in r := (x,y) :: !r ; y
-    | Some y -> y
   in g
+
+open FStar.Classical
+
+let impl_intro (#p:Type0) (#q:Type0) ($f: (squash p) -> Lemma q) : Lemma (p ==> q)  =
+      give_witness #(p ==> q) (arrow_to_impl (lemma_to_squash_gtot f))
+
+let memo_invariant_valid (#a:eqtype) (#b:Type) (f:a -> Tot b) (r:memo_t a b)
+  : Lemma (invariant #a #b (memo_invariant f r) (fun _ -> True) (fun x y -> y == f x) #(fun _ -> memo_invariant f r) #(fun x _ y h1 -> memo_invariant f r h1 /\ y == f x) (memo f r))
+= let p = (memo_invariant f r) in
+  let pre_pure = (fun _ -> True) in
+  let post_pure = (fun x y -> y == f x) in
+  let pre = (fun _ -> memo_invariant f r) in
+  let post = (fun x _ y h1 -> memo_invariant f r h1 /\ y == f x) in
+  let f0 = f in
+  let f = (memo f r) in
+  let stuff (s1 s2:heap) (_:squash (p s1 /\ p s2)) (x:a) (w:squash (pre_pure x))
+    : Lemma (fst (reify (f x) s1) == fst (reify (f x) s2)) =
+    let _ = reify (f x) s1 in
+    let _  = reify (f x) s2 in
+    ()
+  in
+  (* let h0 s1 s2 h1 : Lemma (forall x. pre_pure x ==> (fst (reify (f x) s1) == fst (reify (f x) s2))) = *)
+  (*   forall_intro (fun x -> impl_intro (stuff s1 s2 h1 x)) *)
+  (* in *)
+  (* let h1 s1 s2 : Lemma (p s1 /\ p s2 ==> (forall x. pre_pure x ==> (fst (reify (f x) s1) == fst (reify (f x) s2)))) = impl_intro (h0 s1 s2) in *)
+  (* forall_intro_2 h1 ; *)
+  assert (forall x s. (p s /\ pre_pure x) ==> pre x s) ;
+  assert (forall x s1 s2 y. (p s1 /\ post x s1 y s2) ==> (p s2 /\ post_pure x y)) ;
+  assume (forall s1 s2. p s1 /\ p s2 ==> (forall x. pre_pure x ==> fst (reify (f x) s1) == fst (reify (f x) s2)))
+
+  (* Eat up mre than 6G of ram... *)
+  (* assert_by_tactic *)
+  (*   (forall s1 s2. p s1 /\ p s2 ==> (forall x. pre_pure x ==> fst (reify (f x) s1) == fst (reify (f x) s2))) *)
+  (*   (s1 <-- forall_intro ; *)
+  (*    s2 <-- forall_intro ; *)
+  (*    h1 <-- implies_intro ; *)
+  (*    x <-- forall_intro ; *)
+  (*    h2 <-- implies_intro ; *)
+  (*    apply_lemma (quote stuff) ; *)
+  (*    fail "") ; *)
+
+let memo_invariant_valid' (#a:eqtype) (#b:Type) (f:a -> Tot b)
+    : Lemma (forall (r:memo_t a b). invariant #a #b (memo_invariant f r) (fun _ -> True) (fun x y -> y == f x) #(fun _ -> memo_invariant f r) #(fun x _ y h1 -> memo_invariant f r h1 /\ y == f x) (memo f r))
+= forall_intro (memo_invariant_valid f)
+
+let pure_memo (#a:eqtype) (#b:Type) (f:a -> Tot b) : Pure (a -> Tot b)(requires True) (ensures (fun g -> forall x. g x == f x))=
+  memo_invariant_valid' f ;
+  erase_st #a #b (memo_invariant f) (fun _ -> True) (fun x y -> y == f x) #(fun r _ -> memo_invariant f r) #(fun r x _ y h1 -> memo_invariant f r h1 /\ y == f x) (memo f) (memo_initializer f)
